# 定积分题目与解析

---

## **第一题**

**问题：**
$$
\int_0^{\frac{\pi}{4}} \ln(1+\tan x) dx
$$

**解：**
令 $x = \frac{\pi}{4}-t$，则 $dx = -dt$。当 $x=0$ 时，$t=\frac{\pi}{4}$；当 $x=\frac{\pi}{4}$ 时，$t=0$。

原式 $(I) = \int_{\frac{\pi}{4}}^0 \ln(1+\tan(\frac{\pi}{4}-t)) (-dt) = \int_0^{\frac{\pi}{4}} \ln\left(1 + \frac{\tan\frac{\pi}{4}-\tan t}{1+\tan\frac{\pi}{4}\tan t}\right) dt$

$= \int_0^{\frac{\pi}{4}} \ln\left(1 + \frac{1-\tan t}{1+\tan t}\right) dt$

$= \int_0^{\frac{\pi}{4}} \ln\left(\frac{1+\tan t + 1-\tan t}{1+\tan t}\right) dt$

$= \int_0^{\frac{\pi}{4}} \ln\left(\frac{2}{1+\tan t}\right) dt = \int_0^{\frac{\pi}{4}} (\ln 2 - \ln(1+\tan t)) dt$

$= \int_0^{\frac{\pi}{4}} \ln 2 dt - \int_0^{\frac{\pi}{4}} \ln(1+\tan t) dt$

$= \frac{\pi}{4} \ln 2 - I$

移项可得 $2I = \frac{\pi}{4} \ln 2$，所以 $I = \frac{\pi}{8} \ln 2$。

---

## **第二题**

**问题：**
$$
\int_0^1 \frac{\ln(1+x)}{1+x^2} dx
$$

**解：**
令 $x = \tan\theta$，则 $dx = \sec^2\theta d\theta$。当 $x=0$ 时，$\theta=0$；当 $x=1$ 时，$\theta=\frac{\pi}{4}$。

原式 $= \int_0^{\frac{\pi}{4}} \frac{\ln(1+\tan\theta)}{1+\tan^2\theta} \sec^2\theta d\theta$

由于 $1+\tan^2\theta = \sec^2\theta$，上式简化为：

$= \int_0^{\frac{\pi}{4}} \ln(1+\tan\theta) d\theta$

由第一题结论，原式 $= \frac{\pi}{8} \ln 2$。

---

## **第三题**

**问题：**
$$
\int_0^1 \frac{\arctan x}{1+x} dx
$$

**解：**
$$
\int_0^1 \frac{\arctan x}{1+x} dx = \left[ \arctan x \cdot \ln(1+x) \right]_0^1 - \int_0^1 \frac{\ln(1+x)}{1+x^2} dx
$$

$$
= \left( \frac{\pi}{4}\ln 2 - 0 \right) - \frac{\pi}{8}\ln 2
$$

$$
= \frac{\pi}{8}\ln 2
$$

---

## **第四题**

**问题：**
$$
\int_{\frac{1}{2}}^2 \left(1+x-\frac{1}{x}\right) e^{x+\frac{1}{x}} dx = \int_0^2 \left(\frac{1}{2}+\frac{1}{2}x\right) e^{x+\frac{1}{2}x^2} dx
$$

**解法一：**
首先计算一个不定积分部分：
$$
\int (1-\frac{1}{x^2})e^{x+\frac{1}{x}} dx = \int e^{x+\frac{1}{x}} d\left(x+\frac{1}{x}\right) = e^{x+\frac{1}{x}} + C
$$
对原式进行拆分和分部积分：
原式
$$
= \int_\frac{1}{2}^2 e^{x+\frac{1}{x}} dx + \int_\frac{1}{2}^2 \left(x-\frac{1}{x}\right)e^{x+\frac{1}{x}} dx
$$

$$= \int_\frac{1}{2}^2 e^{x+\frac{1}{x}} dx + \left[ xe^{x+\frac{1}{x}} \right]_\frac{1}{2}^2 - \int_\frac{1}{2}^2 e^{x+\frac{1}{x}} dx = \frac{3}{2}e^{\frac{5}{2}}
$$

**解法二：**
原式
$$
= \int_\frac{1}{2}^2 e^{x+\frac{1}{x}} dx + \int_\frac{1}{2}^2 \left(x-\frac{1}{x}\right)e^{x+\frac{1}{x}} dx
$$

$$
= \left[ xe^{x+\frac{1}{x}} \right]_\frac{1}{2}^2 - \int_\frac{1}{2}^2 x \left(1 - \frac{1}{x^2}\right)e^{x+\frac{1}{x}} dx + \int_\frac{1}{2}^2 \left(x-\frac{1}{x}\right)e^{x+\frac{1}{x}} dx
$$

$$
= \left[ xe^{x+\frac{1}{x}} \right]_\frac{1}{2}^2 = \frac{3}{2}e^{\frac{5}{2}}
$$
